\question{(B2.1)}{
    If $a^2 + bc < 0$, let $\omega > 0$ be the real such that
    $\omega^2 = -(a^2 + bc)$.
    Prove that
    \[
        e^A = \cos \omega I + \frac{\sin \omega}{\omega} A.
    \]
}
\begin{proof}
    \begin{align*}
        A^0 & =
        \begin{pmatrix}
            1 & 0 \\
            0 & 1
        \end{pmatrix} \\
        A^2 & =
        \begin{pmatrix}
            a^2 + cb & ab - ba \\
            ca - ac & cb + a^2
        \end{pmatrix}
        =
        \begin{pmatrix}
            a^2 + cb & 0 \\
            0 & a^2 + cb
        \end{pmatrix}
        = (a^2 + cb)
        \begin{pmatrix}
            1 & 0 \\
            0 & 1
        \end{pmatrix}
        \\
        A^3 & =
        \begin{pmatrix}
            a(a^2 + cb) & b(a^2 + cb) \\
            c(a^2 + cb) & -a(a^2 + cb)
        \end{pmatrix}
        = (a^2 + cb)
        \begin{pmatrix}
            a & b \\
            c & -a
        \end{pmatrix}
        \\
        A^4 & = (a^2 + cb)^2
        \begin{pmatrix}
            1 & 0 \\
            0 & 1
        \end{pmatrix} \\
        etc...
    \end{align*}
    It's clear that these matrices follow the familiar pattern of $e^A = \cos(\theta)I - \sin(\theta)J$, however, we have
    a small issue in that the power for the $sin$ piece is incorrect for our power series. This can be remedied by
    multiplying by $\frac{(a^2 + cb)}{(a^2 + cb)}$. This results in
    \[
        e^A = I + \frac{A^2}{2!} + \cdots + \frac{(a^2 + cb)}{(a^2 + cb)}\frac{A}{3!} + \cdots = \cos(a^2 + cb)I + \frac{\sin(a^2 + cb)}{(a^2 + cb)}A = \cos(\omega)I + \frac{\sin(\omega)}{\omega}A
    \]
    as desired.
\end{proof}
\newpage
